towards reconciling secure_api/hkdf and tls/Hashing

secure_api/hkdf/Crypto.HKDF.fst
@@ -1,5 +1,7 @@
 module Crypto.HKDF
 
+/// 18-03-04 to be compared to Hashing.HKDF, salvaged as a spec 
+
 module ST = FStar.HyperStack.ST
 open FStar.HyperStack.All
 
@@ -9,6 +11,8 @@ open FStar.HyperStack
 open FStar.HyperStack.ST
 open FStar.Buffer
 open FStar.UInt32
+
+open Crypto.Hash 
 
 (* Definition of aliases for modules *)
 module U8 = FStar.UInt8
@@ -23,31 +27,19 @@ let uint64_t  = FStar.UInt64.t
 let uint32_p = Buffer.buffer uint32_t
 let uint8_p  = Buffer.buffer uint8_t
 
-type alg = HMAC.alg
+type alg = Hash.alg13
 
 // ADL July 4
 #set-options "--lax"
-(* Define HKDF Extraction function *)
-val hkdf_extract :
-  a       : alg ->
-  prk     : uint8_p{length prk = v (HMAC.hash_size a)} ->
-  salt    : uint8_p ->
-  saltlen : uint32_t{v saltlen = length salt} ->
-  ikm     : uint8_p ->
-  ikmlen  : uint32_t{v ikmlen = length ikm} ->
-  Stack unit
-        (requires (fun h0 -> live h0 prk /\ live h0 salt /\ live h0 ikm))
-        (ensures  (fun h0 r h1 -> live h1 prk /\ modifies_1 prk h0 h1))
 
 let hkdf_extract a prk salt saltlen ikm ikmlen =
-  HMAC.hmac a prk salt saltlen ikm ikmlen
-
+  HMAC.compute a prk salt saltlen ikm ikmlen
 
 [@"c_inline"]
 private val hkdf_expand_inner:
   a       : alg ->
   state   : uint8_p ->
-  prk     : uint8_p {v (HMAC.hash_size a) <= length prk} ->
+  prk     : uint8_p {Hash.tagLength a <= length prk} ->
   prklen  : uint32_t {v prklen = length prk} ->
   info    : uint8_p ->
   infolen : uint32_t {v infolen = length info} ->
@@ -65,7 +57,7 @@ let rec hkdf_expand_inner a state prk prklen info infolen n i =
 
   (* Recompute the sizes and position of the intermediary objects *)
   (* Note: here we favour readability over efficiency *)
-  let size_Ti  = HMAC.hash_size a in
+  let size_Ti  = Hash.tagLen  a in
   let size_Til = size_Ti +^ infolen +^ 1ul in
   let size_T = U32.mul_mod n size_Ti in
 
@@ -73,18 +65,18 @@ let rec hkdf_expand_inner a state prk prklen info infolen n i =
   let pos_Til = size_Ti in
   let pos_T = pos_Til +^ size_Til in
 
-  (* Retreive the memory for local computations. state =  Ti | Til | T *)
+  (* Retrieve the memory for local computations. state =  Ti | Til | T *)
   let ti = Buffer.sub state pos_Ti size_Ti in
   let til = Buffer.sub state pos_Til size_Til in
   let t = Buffer.sub state pos_T size_T in
 
-  if (i =^ 1ul) then begin
+  if i = 1ul then begin
 
     Buffer.blit info 0ul til 0ul infolen;
     Buffer.upd til infolen (Int.Cast.uint32_to_uint8 i);
 
     (* Compute the mac of to get block Ti *)
-    HMAC.hmac a ti prk prklen til (infolen +^ 1ul);
+    HMAC.compute a ti prk prklen til (infolen +^ 1ul);
 
     (* Store the resulting block in T *)
     Buffer.blit ti 0ul t 0ul size_Ti;
@@ -92,7 +84,7 @@ let rec hkdf_expand_inner a state prk prklen info infolen n i =
     (* Recursive call *)
     hkdf_expand_inner a state prk prklen info infolen n (i +^ 1ul) end
 
-  else if (i <=^ n) then begin
+  else if i <=^ n then begin
 
     (* Concatenate T(i-1) | Info | i *)
     Buffer.blit ti 0ul til 0ul size_Ti;
@@ -100,7 +92,7 @@ let rec hkdf_expand_inner a state prk prklen info infolen n i =
     Buffer.upd til (size_Til -^ 1ul) (Int.Cast.uint32_to_uint8 i);
 
     (* Compute the mac of to get block Ti *)
-    HMAC.hmac a ti prk prklen til size_Til;
+    HMAC.compute a ti prk prklen til size_Til;
 
     (* Store the resulting block in T *)
     let pos = U32.mul_mod (i -^ 1ul) size_Ti in
@@ -113,42 +105,25 @@ let rec hkdf_expand_inner a state prk prklen info infolen n i =
   (* Pop the memory frame *)
   (**) pop_frame()
 
-(* Define HKDF Expand function *)
-val hkdf_expand :
-  a       : alg ->
-  okm     : uint8_p ->
-  prk     : uint8_p {v (HMAC.hash_size a) <= length prk} ->
-  prklen  : uint32_t {v prklen <= length prk} ->
-  info    : uint8_p ->
-  infolen : uint32_t {v infolen <= length info} ->
-  len     : uint32_t {v len <= length okm
-                    /\ v len <= (255 * U32.v (HMAC.hash_size a))
-                    /\ (U32.v len / U32.v (HMAC.hash_size a) + 1) <= length okm} ->
-  Stack unit
-        (requires (fun h0 -> live h0 okm /\ live h0 prk /\ live h0 info))
-        (ensures  (fun h0 r h1 -> live h1 okm /\ modifies_1 okm h0 h1))
 
 let hkdf_expand a okm prk prklen info infolen len =
-
-  (* Push a new memory frame *)
-  (**) push_frame ();
-
+  push_frame ();
+  let size_Ti = tagLen a in 
   (* Compute the number of blocks necessary to compute the output *)
-  let size_Ti = HMAC.hash_size a in
   // ceil
-  let n_0 = if U32.(rem len size_Ti) = 0ul then 0ul else 1ul in
-  let n = U32.(div len size_Ti) +^ n_0 in
+  let n_0 = if len %^ size_Ti = 0ul then 0ul else 1ul in
+  let n = len /^ size_Ti +^ n_0 in
 
   (* Describe the shape of memory used by the inner recursive function *)
-  let size_T = U32.mul_mod n size_Ti in
   let size_Til = size_Ti +^ infolen +^ 1ul in
+  let size_T = n *^ size_Ti in
 
   let pos_Ti = 0ul in
   let pos_Til = size_Ti in
   let pos_T = pos_Til +^ size_Til in
 
-  (* Allocate memory for inner expension: state =  Ti | Til | T *)
-  let state = Buffer.create 0uy (size_Ti +^ size_Til +^ size_T) in
+  (* Allocate memory for inner expansion state: Ti @| Til @| T *)
+  let state = Buffer.create 0uy (tagLen a +^ size_Til +^ size_T) in
 
   (* Call the inner expension function *)
   if n >^ 0ul then
@@ -160,5 +135,70 @@ let hkdf_expand a okm prk prklen info infolen len =
   (* Redundant copy the desired part of T *)
   Buffer.blit _T 0ul okm 0ul len;
 
-  (* Pop the memory frame *)
-  (**) pop_frame()
+  pop_frame()
+
+
+//18-03-05 I'd rather simplify a simpler implementation, closer to the spec,
+//18-03-05 We could make do with fewer loop variables if it helps with C.Loops
+private val hkdf_expand_loop: 
+  a       : alg13 ->
+  okm     : bptr ->
+  prk     : bptr {disjoint okm prk} ->
+  prklen  : bptrlen prk ->
+  infolen : UInt32.t -> 
+  len     : bptrlen okm { v len <= 255 * tagLength a } ->
+  hashed  : lbptr (tagLength a + v infolen + 1) {disjoint hashed okm /\ disjoint hashed prk} ->
+  i       : UInt8.t {i <> 0uy} ->
+  Stack unit
+  (requires fun h0 -> 
+    live h0 okm /\ live h0 prk /\ live h0 hashed)
+  (ensures  fun h0 r h1 -> 
+    live h1 okm /\ modifies_2 okm hashed h0 h1 /\ (
+    let prk = as_seq h0 prk in 
+    let info = as_seq h0 (Buffer.sub hashed (tagLen a) infolen) in 
+    let last = if i = 1uy then Seq.createEmpty else as_seq h0 (Buffer.sub hashed 0ul (tagLen a)) in 
+    let okm = as_seq h1 okm in 
+    okm =  expand0 a prk info (v len) (UInt8.v i) last))
+
+
+[@"c_inline"]
+let rec hkdf_expand_loop a okm prk prklen infolen len hashed i =
+  push_frame ();
+
+  let tlen = tagLen a in 
+  let tag = Buffer.sub hashed 0ul tlen in 
+
+  // derive one more block
+  Buffer.upd hashed (tlen +^ infolen) i;
+  if i = 1uy then (
+    // the first input is shorter, does not include the chaining block
+    let len1 = infolen +^ 1ul in 
+    let hashed1 = Buffer.sub hashed tlen len1 in
+    HMAC.compute a hashed prk prklen hashed1 len1 )
+  else
+    HMAC.compute a hashed prk prklen hashed (tlen +^ infolen +^ 1ul);
+
+  // copy it to the result, and iterate if required
+  if len <=^ tlen then 
+    Buffer.blit tag 0ul okm 0ul len 
+  else (
+    Buffer.blit tag 0ul okm 0ul tlen;
+    let len = len -^ tlen in 
+    let okm = Buffer.sub okm tlen len in 
+    let i = FStar.UInt8.(i +^ 1uy) in 
+    hkdf_expand_loop a okm prk prklen infolen len hashed i);
+    
+  pop_frame()
+
+
+[@"c_inline"]
+let hkdf_expand_alt a okm prk prklen info infolen len = 
+  push_frame();
+  let tlen = tagLen a in 
+  let hashed = Buffer.create 0uy (tlen +^ infolen +^ 1ul) in 
+  Buffer.blit info 0ul hashed tlen infolen; 
+  hkdf_expand_loop a okm prk prklen infolen len hashed 1uy;
+  pop_frame()
+
+
+
