secure_api/hkdf/Crypto.HMAC.fst
@@ -1,189 +1,129 @@
-(* Agile HKDF *)
+(* Agile HMAC *)
 module Crypto.HMAC
 
-module ST = FStar.HyperStack.ST
+/// Agile specification
+
+type alg = Hash.alg13
+
+open FStar.Seq 
+
+noextract 
+let wrap (a:alg) (key: bseq{Seq.length key <= maxLength a}): 
+  Tot (lbseq (blockLength a))
+= 
+  let key0 = if length key <= blockLength a then key else hash a key in 
+  let padding = blockLength a - length key0 in 
+  key0 @| Seq.create padding 0uy
+
+noextract 
+let xor k v = Spec.Loops.seq_map (fun x -> FStar.UInt8.logxor x v) k
+
+// [noextract] incompatible with interfaces?!
+let hmac a key data =
+  let k = wrap a key in 
+  let h1 = hash a (xor k 0x36uy @| data) in 
+  let h2 = hash a (xor k 0x5cuy @| h1) in 
+  h2
+
+
+/// Agile implementation, relying on using 3 variants of SHA2
+/// supported by HACL*.
+
 open FStar.HyperStack.All
-
-open FStar.HyperStack
 open FStar.Buffer
-open Buffer.Utils
-
-module HS = FStar.HyperStack
-
 open FStar.UInt32
-open Crypto.Symmetric.Bytes
-open Crypto.Indexing
 
-open C.Loops
-
-(* Definition of aliases for modules *)
-module U8 = FStar.UInt8
-module U32 = FStar.UInt32
-module U64 = FStar.UInt64
-
-module Spec_H256 = Spec.SHA2_256
-module H256 = Hacl.Hash.SHA2_256
-module Spec_H384 = Spec.SHA2_384
-module H384 = Hacl.Hash.SHA2_384
-module Spec_H512 = Spec.SHA2_512
-module H512 = Hacl.Hash.SHA2_512
-
-module Spec_HMAC256 = Spec.HMAC.SHA2_256
-
-private let uint8_t  = FStar.UInt8.t
-private let uint32_t = FStar.UInt32.t
-private let uint32_p = Buffer.buffer uint32_t
-private let uint8_p  = Buffer.buffer uint8_t
-private let uint64_t = FStar.UInt64.t
-private let uint64_p = Buffer.buffer uint64_t
-
-//
-// HMAC-SHA2-256
-//
+module ST = FStar.HyperStack.ST
 
 // ADL lax prototype for QUIC deadline
-#set-options "--lax"
+// 18-03-04 restructured
 
-//#reset-options "--max_fuel 0 --z3rlimit 10"
-let xor_bytes_inplace a b len =
-  C.Loops.in_place_map2 a b len (fun x y -> U8.logxor x y)
-
-type alg =
-  | SHA256
-  | SHA384
-  | SHA512
-
-//#reset-options "--initial_ifuel 2 --initial_fuel 0 --z3rlimit 20"
-let block_size : alg -> Tot uint32_t = function
-  | SHA256 -> H256.size_block
-  | SHA384 -> H384.size_block
-  | SHA512 -> H512.size_block
-
-let hash_size: alg -> Tot uint32_t = function
-  | SHA256 -> H256.size_hash
-  | SHA384 -> H384.size_hash_final // Note that `size_hash` is 64, not 48
-  | SHA512 -> H512.size_hash
-
-// FIXME(adl): hash state allocation
-// The type of state a is a buffer of uint32 for SHA256
-// but a buffer of uint64 for SHA384 and SHA512
-// This is hard to do in KreMLin (see Crypto.Symmetric.PRF)
-// Instead we fake a u64[n] by allocation a u32[2*n]
-// and rely on the implicit cast in C
-inline_for_extraction let state_size: alg -> Tot uint32_t = function
-  | SHA256 -> H256.size_state
-  | SHA384 -> U32.mul 2ul H384.size_state
-  | SHA512 -> U32.mul 2ul H512.size_state
-
-//#reset-options "--initial_ifuel 2 --initial_fuel 2 --z3rlimit 30"
-noextract let max_byte_length : alg -> Tot nat = function
-  | SHA256 -> Spec_H256.max_input_len_8
-  | SHA384 -> Spec_H384.max_input_len_8
-  | SHA512 -> Spec_H512.max_input_len_8
-
-//#reset-options "--initial_fuel 0 --initial_ifuel 0 --z3rlimit 20"
-let correct_wrap_key (a:alg)
-  (key:Seq.seq uint8_t{Seq.length key < max_byte_length a})
-  (wrapped:Seq.seq uint8_t{Seq.length wrapped = v (block_size a)}) : GTot Type =
-  match a with
-  | SHA256 -> Spec_HMAC256.wrap_key key == wrapped
-  | SHA384 -> True // Spec missing
-  | SHA512 -> True // Spec missing
-
-let correct_agile_hash (a:alg)
-  (input:Seq.seq uint8_t{Seq.length input < max_byte_length a})
-  (digest:Seq.seq uint8_t{Seq.length digest = v (hash_size a)})
-  : GTot Type =
-  match a with
-  | SHA256 -> Spec_H256.hash input == digest
-  | SHA384 -> Spec_H384.hash input == digest
-  | SHA512 -> Spec_H512.hash input == digest
-
+(* we rely on the output being zero-initialized in case the key is less than a block *)
 [@"substitute"]
 val wrap_key:
-  a      : alg ->
-  output : uint8_p  {length output = v (block_size a)} ->
-  key    : uint8_p  {disjoint output key} ->
-  len    : uint32_t {v len = length key /\ v len < max_byte_length a} ->
+  a: alg ->
+  output: lbptr (blockLength a) ->
+  key: bptr {length key <= maxLength a /\ disjoint output key} ->
+  len: UInt32.t {v len = length key} ->
   Stack unit
-    (requires (fun h -> live h output /\ live h key /\
-      (as_seq h output) == Seq.create (v (block_size a)) 0uy))
-    (ensures  (fun h0 _ h1 -> live h1 output /\ live h1 key /\ live h0 output /\ live h0 key
-      /\ modifies_1 output h0 h1
-      /\ as_seq h0 output == Seq.create (v (block_size a)) 0uy
-      /\ correct_wrap_key a (as_seq h0 key) (as_seq h1 output)))
+    (requires (fun h0 -> 
+      live h0 output /\ live h0 key /\
+      as_seq h0 output == Seq.create (blockLength a) 0uy ))
+    (ensures  (fun h0 _ h1 -> 
+      live h1 output /\ live h1 key /\ live h0 output /\ live h0 key /\
+      as_seq h0 output == Seq.create (blockLength a) 0uy /\
+      modifies_1 output h0 h1 /\
+      as_seq h1 output = wrap a (as_seq h0 key) ))
 
-let agile_hash (a:alg) (output:uint8_p{length output = v (hash_size a)})
-  (input:uint8_p{length input < max_byte_length a /\ disjoint output input})
-  (len:uint32_t{v len = length output})
-  : Stack unit
-  (requires fun h -> live h input /\ live h output
-    /\ (as_seq h output) == Seq.create (v (hash_size a)) 0uy)
-  (ensures fun h0 () h1 -> live h1 output /\ live h1 input
-    /\ modifies_1 output h0 h1
-    /\ as_seq h1 input == as_seq h0 input
-    /\ correct_agile_hash a (as_seq h1 input) (as_seq h1 output))
-  =
-  match a with
-  | SHA256 -> H256.hash output input len
-  | SHA384 -> H384.hash output input len
-  | SHA512 -> H512.hash output input len
+// replaced by [H.compute]; not sure why it required pre-zeroing-out the result.
+// let agile_hash (a:alg) (output:uint8_p{length output = tagLength a})
+//   (input:uint8_p{length input < maxLength a /\ disjoint output input})
+//   (len:uint32_t{v len = length output})
+//   : Stack unit
+//   (requires fun h -> live h input /\ live h output
+//     /\ (as_seq h output) == Seq.create (tagLength a) 0uy)
+//   (ensures fun h0 () h1 -> live h1 output /\ live h1 input
+//     /\ modifies_1 output h0 h1
+//     /\ as_seq h1 input == as_seq h0 input
+//     /\ correct_agile_hash a (as_seq h1 input) (as_seq h1 output))
+//   =
+//   match a with
+//   | SHA256 -> Hacl.Hash.SHA2_256.hash output input len
+//   | SHA384 -> Hacl.Hash.SHA2_384.hash output input len
+//   | SHA512 -> Hacl.Hash.SHA2_512..hash output input len
 
 //#reset-options "--max_fuel 0  --z3rlimit 250"
 [@"substitute"]
 let wrap_key a output key len =
  (**) let h0 = ST.get () in
-  if len <=^ block_size a then
+  if len <=^ blockLen a then
    begin
-    (**) assert(v (block_size a) - v len >= 0);
-    (**) assert(as_seq h0 output == Seq.create (v (block_size a)) 0uy);
+    (**) assert(v (blockLen a) - v len >= 0);
+    (**) assert(as_seq h0 output == Seq.create (v (blockLen a)) 0uy);
     Buffer.blit key 0ul output 0ul len;
     (**) let h1 = ST.get () in
     (**) Seq.lemma_eq_intro (Seq.slice (as_seq h1 output) 0 (v len)) (as_seq h0 key);
     (**) assert(Seq.slice (as_seq h1 output) 0 (v len) == as_seq h0 key);
-    (**) Seq.lemma_eq_intro (Seq.slice (as_seq h1 output) (v len) (v (block_size a))) (Seq.create (v (block_size a) - v len) 0uy);
-    (**) assert(Seq.slice (as_seq h1 output) (v len) (v (block_size a)) == Seq.create (v (block_size a) - v len) 0uy);
-    (**) Seq.lemma_eq_intro (as_seq h1 output) (Seq.append (as_seq h0 key) (Seq.create (v (block_size a) - v len) 0uy));
-    (**) assert(as_seq h1 output == Seq.append (as_seq h0 key) (Seq.create (v (block_size a) - v len) 0uy))
+    (**) Seq.lemma_eq_intro (Seq.slice (as_seq h1 output) (v len) (v (blockLen a))) (Seq.create (v (blockLen a) - v len) 0uy);
+    (**) assert(Seq.slice (as_seq h1 output) (v len) (v (blockLen a)) == Seq.create (v (blockLen a) - v len) 0uy);
+    (**) Seq.lemma_eq_intro (as_seq h1 output) (Seq.append (as_seq h0 key) (Seq.create (v (blockLen a) - v len) 0uy));
+    (**) assert(as_seq h1 output == Seq.append (as_seq h0 key) (Seq.create (v (blockLen a) - v len) 0uy))
    end
   else
    begin
-    (**) assert(v (block_size a) - v (hash_size a) >= 0);
-    (**) assert(as_seq h0 output == Seq.create (v (block_size a)) 0uy);
-    (**) Seq.lemma_eq_intro (Seq.slice (as_seq h0 output) 0 (v (hash_size a))) (Seq.create (v (hash_size a)) 0uy);
-    (**) assert(Seq.slice (as_seq h0 output) 0 (v (hash_size a)) == Seq.create (v (hash_size a)) 0uy);
-    (**) Seq.lemma_eq_intro (Seq.slice (as_seq h0 output) (v (hash_size a)) (v (block_size a))) (Seq.create (v (block_size a) - v (hash_size a)) 0uy);
-    (**) assert(Seq.slice (as_seq h0 output) (v (hash_size a)) (v (block_size a)) == Seq.create (v (block_size a) - v (hash_size a)) 0uy);
-    let nkey = Buffer.sub output 0ul (hash_size a) in
-    agile_hash a nkey key len
-//    (**) let h1' = ST.get () in
-//    (**) assert(as_seq h1' nkey == );
-//    (**) assert(Seq.slice (as_seq h1' output) 0 (v (hash_size a)) == Spec_Hash.hash (as_seq h0 key));
-//    (**) no_upd_lemma_1 h0 h1' (Buffer.sub output 0ul (hash_size a)) (Buffer.sub output (hash_size a) ((block_size a) -^ (hash_size a)));
-//    (**) Seq.lemma_eq_intro (Seq.slice (reveal_sbytes (as_seq h1' output)) (v (hash_size a)) (v (block_size a))) (Seq.create (v (block_size a) - v (hash_size a)) 0uy);
-//    (**) assert(Seq.slice (reveal_sbytes (as_seq h1' output)) (v (hash_size a)) (v (block_size a)) == Seq.create (v (block_size a) - v (hash_size a)) 0uy);
-//    (**) Seq.lemma_eq_intro (reveal_sbytes (as_seq h1' output)) (Seq.append (reveal_sbytes (as_seq h1' nkey)) (Seq.create (v (block_size a) - v (hash_size a)) 0uy));
-//    (**) assert(reveal_sbytes (as_seq h1' output) == Seq.append (reveal_sbytes (as_seq h1' nkey)) (Seq.create (v (block_size a) - v (hash_size a)) 0uy))
+    (**) assert(v (blockLen a) - tagLength a >= 0);
+    (**) assert(as_seq h0 output == Seq.create (v (blockLen a)) 0uy);
+    (**) Seq.lemma_eq_intro (Seq.slice (as_seq h0 output) 0 (tagLength a)) (Seq.create (tagLength a) 0uy);
+    (**) assert(Seq.slice (as_seq h0 output) 0 (tagLength a) == Seq.create (tagLength a) 0uy);
+    (**) Seq.lemma_eq_intro (Seq.slice (as_seq h0 output) (tagLength a) (v (blockLen a))) (Seq.create (v (blockLen a) - tagLength a) 0uy);
+    (**) assert(Seq.slice (as_seq h0 output) (tagLength a) (v (blockLen a)) == Seq.create (v (blockLen a) - tagLength a) 0uy);
+    let nkey = Buffer.sub output 0ul (tagLen a) in
+    Hash.compute a len key nkey
+    (**) //let h1' = ST.get () in
+    (**) //assert(as_seq h1' nkey == );
+    (**) //assert(Seq.slice (as_seq h1' output) 0 (tagLength a) == Spec_Hash.hash (as_seq h0 key));
+    (**) //no_upd_lemma_1 h0 h1' (Buffer.sub output 0ul (tagLen a)) (Buffer.sub output (tagLen a) blockLen a) -^ (tagLen a)));
+    (**) //Seq.lemma_eq_intro (Seq.slice (reveal_sbytes (as_seq h1' output)) (tagLength a) (v (blockLen )) (Seq.create (v (blockLen a) - tagLength a) 0uy);
+    (**) //assert(Seq.slice (reveal_sbytes (as_seq h1' output)) (tagLength a) (v (blockLen a)) == Seq.create (v (blockLen a) - tagLength a) 0uy);
+    (**) //Seq.lemma_eq_intro (reveal_sbytes (as_seq h1' output)) (Seq.append (reveal_sbytes (as_seq h1' nkey)) (Seq.create (v (blockLen a) - tagLength a) 0uy));
+    (**) //assert(reveal_sbytes (as_seq h1' output) == Seq.append (reveal_sbytes (as_seq h1' nkey)) (Seq.create (v (blockLen a) - tagLength a) 0uy))
    end
 
+(* should not be necessary 
 //#reset-options " --initial_fuel 1 --max_fuel 1 --initial_ifuel 1 --max_ifuel 1 --z3rlimit 10"
 let counter_pos: alg -> Tot uint32_t = function
-  | SHA256 -> H256.pos_count_w
-  | SHA384 -> H384.pos_count_w
-  | SHA512 -> H512.pos_count_w
+  | SHA256 -> Hacl.Hash.SHA2_256.pos_count_w
+  | SHA384 -> Hacl.Hash.SHA2_384.pos_count_w
+  | SHA512 -> Hacl.Hash.SHA2_512.pos_count_w
 
 //#reset-options "--initial_fuel 1 --max_fuel 1 --initial_ifuel 1 --max_ifuel 1 --z3rlimit 10"
 let counter_size: alg -> Tot uint32_t = function
-  | SHA256 -> H256.size_count_w
-  | SHA384 -> H384.size_count_w
-  | SHA512 -> H512.size_count_w
+  | SHA256 -> Hacl.Hash.SHA2_256.size_count_w
+  | SHA384 -> Hacl.Hash.SHA2_384.size_count_w
+  | SHA512 -> Hacl.Hash.SHA2_512..size_count_w
+*)
 
-type state (a:alg) =
-  (match a with
-  | SHA256 -> st:uint32_p{length st = v (H256.size_state)}
-  | SHA384 -> st:uint64_p{length st = v (H384.size_state)}
-  | SHA512 -> st:uint64_p{length st = v (H512.size_state)})
-
+(* usage? 
 //#reset-options "--max_fuel 0  --z3rlimit 50"
 val lemma_alloc:
   a: alg ->
@@ -195,20 +135,21 @@ val lemma_alloc:
       let counter = Seq.index seq_counter 0 in
       U32.v counter = 0))
 let lemma_alloc a s = ()
+*)
 
 //#reset-options "--max_fuel 0  --z3rlimit 20"
 [@"substitute"]
 val hmac_part1:
-  a    : alg ->
-  s2   : uint8_p {length s2 = v (block_size a)} ->
-  data : uint8_p  {length data + v (block_size a) < pow2 32 /\ disjoint data s2} ->
-  len  : uint32_t {length data = v len} ->
+  a: alg ->
+  s2: lbptr (blockLength a) ->
+  data: bptr {length data + blockLength a  < pow2 32 /\ disjoint data s2} ->
+  len: UInt32.t {length data = v len} ->
   Stack unit
-        (requires (fun h ->  live h s2 /\ live h data))
+        (requires (fun h0 ->  live h0 s2 /\ live h0 data))
         (ensures  (fun h0 _ h1 -> live h1 s2 /\ live h0 s2
                              /\ live h1 data /\ live h0 data /\ modifies_1 s2 h0 h1
-                             /\ (let hash0 = Seq.slice (as_seq h1 s2) 0 (v (hash_size a)) in
-                             correct_agile_hash a (Seq.append (as_seq h0 s2) (as_seq h0 data)) hash0)))
+                             /\ (let hash0 = Seq.slice (as_seq h1 s2) 0 (tagLength a) in
+                             hash0 = hash a (Seq.append (as_seq h0 s2) (as_seq h0 data)))))
 
 (*
 let agile_alloc (a:alg) : Stack (st:state a)
@@ -221,61 +162,20 @@ let agile_alloc (a:alg) : Stack (st:state a)
   | SHA512 -> Buffer.create 0uL (state_size a)
 *)
 
-let agile_init (a:alg) (st:state a) : Stack unit
- (requires fun h -> True)
- (ensures fun h0 () h1 -> True)
-  //live h1 st /\ modifies_1 st h0 h1)
- =
- match a with
- | SHA256 -> H256.init st
- | SHA384 -> H384.init st
- | SHA512 -> H512.init st
+//18-03-04 the condition on len was probably false; not also the
+//calling convention has changed.
+// let Hash.update_last (a:alg) (st:state a)
+//   (input:uint8_p {length input = v (blockLen a)})
+//   (len:uint32_t {v len = length input})
+//   : Stack unit (requires fun h -> True)
+//   (ensures fun h0 () h1 -> True)
+//    //live h1 st /\ modifies_1 st h0 h1)
+//   =
+//   match a with
+//   | SHA256 -> Hacl.Hash.SHA2_256.update_last st input len
+//   | SHA384 -> Hacl.Hash.SHA2_384.update_last st input (Int.Cast.uint32_to_uint64 len)
+//   | SHA512 -> Hacl.Hash.SHA2_512..update_last st input (Int.Cast.uint32_to_uint64 len)
 
-let agile_update (a:alg) (st:state a)
-  (input:uint8_p {length input = v (block_size a)})
-  : Stack unit (requires fun h -> True)
-  (ensures fun h0 () h1 -> True)
-   //live h1 st /\ modifies_1 st h0 h1)
-  =
-  match a with
-  | SHA256 -> H256.update st input
-  | SHA384 -> H384.update st input
-  | SHA512 -> H512.update st input
-
-let agile_update_last (a:alg) (st:state a)
-  (input:uint8_p {length input = v (block_size a)})
-  (len:uint32_t {v len = length input})
-  : Stack unit (requires fun h -> True)
-  (ensures fun h0 () h1 -> True)
-   //live h1 st /\ modifies_1 st h0 h1)
-  =
-  match a with
-  | SHA256 -> H256.update_last st input len
-  | SHA384 -> H384.update_last st input (Int.Cast.uint32_to_uint64 len)
-  | SHA512 -> H512.update_last st input (Int.Cast.uint32_to_uint64 len)
-
-let agile_finish (a:alg) (st:state a)
-  (hash:uint8_p {length hash = v (hash_size a)})
-  : Stack unit (requires fun h -> True)
-  (ensures fun h0 () h1 -> True)
-   //live h1 st /\ modifies_1 st h0 h1)
-  =
-  match a with
-  | SHA256 -> H256.finish st hash
-  | SHA384 -> H384.finish st hash
-  | SHA512 -> H512.finish st hash
-
-let agile_update_multi (a:alg) (st:state a)
-  (input:uint8_p {length input % v (block_size a) = 0})
-  (nblocks:uint32_t{op_Multiply (v nblocks) (v (block_size a)) = length input})
-  : Stack unit (requires fun h -> True)
-  (ensures fun h0 () h1 -> True)
-   //live h1 st /\ modifies_1 st h0 h1)
-  =
-  match a with
-  | SHA256 -> H256.update_multi st input nblocks
-  | SHA384 -> H384.update_multi st input nblocks
-  | SHA512 -> H512.update_multi st input nblocks
 
 //#reset-options "--max_fuel 0  --z3rlimit 200"
 [@"substitute"]
@@ -289,39 +189,39 @@ let hmac_part1 a s2 data len =
   // let state0 = Hash.alloc () in
   let state0 = Buffer.create 0ul (state_size a) in
   (**) let h = ST.get() in
-//  (**) lemma_alloc (reveal_h32s (as_seq h state0));
+  (**) //lemma_alloc (reveal_h32s (as_seq h state0));
   (**) no_upd_lemma_0 h0 h s2;
   (**) no_upd_lemma_0 h0 h data;
 
   (* Step 3: append data to "result of step 2" *)
   (* Step 4: apply Hash to "result of step 3" *)
-  (**) assert((block_size a) <> 0ul);
-  (**) Math.Lemmas.lemma_div_mod (v len) (v (block_size a));
-  let n0 = U32.div len (block_size a) in
-  let r0 = U32.rem len (block_size a) in
-  let blocks0 = Buffer.sub data 0ul (n0 *^ (block_size a)) in
-  let last0 = Buffer.offset data (n0 *^ (block_size a)) in
-  (**) Seq.lemma_eq_intro (Seq.slice (as_seq h data) 0 (U32.v (n0 *^ (block_size a)))) (as_seq h blocks0);
-  (**) Seq.lemma_eq_intro (Seq.slice (as_seq h data) (U32.v (n0 *^ (block_size a))) (length data)) (as_seq h last0);
-  agile_init a state0;
-//  (**) let h' = ST.get() in
-//  (**) no_upd_lemma_1 h h' state0 s2;
-//  (**) no_upd_lemma_1 h h' state0 data;
-//  (**) no_upd_lemma_1 h h' state0 blocks0;
-//  (**) no_upd_lemma_1 h h' state0 last0;
-  agile_update a state0 s2;
-//  (**) let h'' = ST.get() in
-//  (**) no_upd_lemma_1 h' h'' state0 blocks0;
-//  (**) no_upd_lemma_1 h' h'' state0 last0;
-  agile_update_multi a state0 blocks0 n0;
-//  (**) let h''' = ST.get() in
-//  (**) no_upd_lemma_1 h'' h''' state0 last0;
-  agile_update_last a state0 last0 r0;
+  (**) assert((blockLen a) <> 0ul);
+  (**) Math.Lemmas.lemma_div_mod (v len) (v (blockLen a));
+  let n0 = len /^ blockLen a in
+  let r0 = len %^ blockLen a in
+  let blocks0 = Buffer.sub data 0ul (n0 *^ (blockLen a)) in
+  let last0 = Buffer.offset data (n0 *^ (blockLen a)) in
+  (**) Seq.lemma_eq_intro (Seq.slice (as_seq h data) 0 (UInt32.v (n0 *^ (blockLen a)))) (as_seq h blocks0);
+  (**) Seq.lemma_eq_intro (Seq.slice (as_seq h data) (UInt32.v (n0 *^ (blockLen a))) (length data)) (as_seq h last0);
+  Hash.init a state0;  
+  (**) //let h' = ST.get() in
+  (**) //no_upd_lemma_1 h h' state0 s2;
+  (**) //no_upd_lemma_1 h h' state0 data;
+  (**) //no_upd_lemma_1 h h' state0 blocks0;
+  (**) //no_upd_lemma_1 h h' state0 last0;
+  Hash.update a state0 s2;
+  (**) //let h'' = ST.get() in
+  (**) //no_upd_lemma_1 h' h'' state0 blocks0;
+  (**) //no_upd_lemma_1 h' h'' state0 last0;
+  Hash.update_multi a state0 blocks0 n0;
+  (**) //let h''' = ST.get() in
+  (**) //no_upd_lemma_1 h'' h''' state0 last0;
+  Hash.update_last a state0 last0 len;
   (**) let h1 = ST.get () in
 
   let h'''' = ST.get() in
-  let hash0 = Buffer.sub s2 0ul (hash_size a) in (* Salvage memory *)
-  agile_finish a state0 hash0; (* s4 = hash (s2 @| data) *)
+  let hash0 = Buffer.sub s2 0ul (tagLen a) in (* Salvage memory *)
+  Hash.extract a state0 hash0; (* s4 = hash (s2 @| data) *)
 //  (**) Spec_Hash.lemma_hash_all_prepend_block (reveal_sbytes (as_seq h0 s2)) (reveal_sbytes (as_seq h0 data));
 
   (* Pop the memory frame *)
@@ -331,14 +231,14 @@ let hmac_part1 a s2 data len =
 //#reset-options "--max_fuel 0  --z3rlimit 20"
 [@"substitute"]
 val hmac_part2:
-  a   : alg ->
-  mac : uint8_p {length mac = v (hash_size a)} ->
-  s5  : uint8_p {length s5 = v (block_size a) /\ disjoint s5 mac} ->
-  s4  : uint8_p {length s4 = v (hash_size a) /\ disjoint s4 mac /\ disjoint s4 s5} ->
+  a: alg ->
+  mac: lbptr (tagLength a) ->
+  s5: lbptr (blockLength a) {disjoint s5 mac} ->
+  s4: lbptr (tagLength a) {disjoint s4 mac /\ disjoint s4 s5} ->
   Stack unit
         (requires (fun h -> True)) //live h mac /\ live h s5 /\ live h s4))
         (ensures  (fun h0 _ h1 -> live h1 mac /\ live h0 mac))
-
+ //TODO spec
  ///\ live h1 s5 /\ live h0 s5
  ///\ live h1 s4 /\ live h0 s4 /\ modifies_1 mac h0 h1
  ///\ (reveal_sbytes (as_seq h1 mac) == Spec_Hash.hash (Seq.append (reveal_sbytes (as_seq h0 s5)) (reveal_sbytes (as_seq h0 s4))))))
@@ -346,13 +246,10 @@ val hmac_part2:
 //#reset-options "--max_fuel 0  --z3rlimit 200"
 [@"substitute"]
 let hmac_part2 a mac s5 s4 =
-  assert_norm(pow2 32 = 0x100000000);
-  let hinit = ST.get() in
-
-  (* Push a new memory frame *)
+  (**) assert_norm(pow2 32 = 0x100000000);
+  (**) let hinit = ST.get() in
   (**) push_frame ();
   (**) let h0 = ST.get () in
-
   (* Allocate memory for the Hash function state *)
   (* let state1 = Hash.alloc () in *)
   let state1 = Buffer.create 0ul (state_size a) in
@@ -363,125 +260,97 @@ let hmac_part2 a mac s5 s4 =
   (**) no_upd_lemma_0 h0 h s5;
   (**) no_upd_lemma_0 h0 h s4;
   (**) no_upd_lemma_0 h0 h mac;
-//  (**) lemma_alloc (reveal_h32s (as_seq h state1));
-  agile_init a state1;
+  (**) //lemma_alloc (reveal_h32s (as_seq h state1));
+  Hash.init a state1;
   (**) let h' = ST.get() in
-//  (**) assert(
-//       let st_h0 = Seq.slice (as_seq h' state1) (U32.v Hash.pos_whash_w) (U32.(v Hash.pos_whash_w + v Hash.size_whash_w)) in
-//       reveal_h32s st_h0 == Spec_Hash.h_0);
+  (**) //assert(let st_h0 = Seq.slice (as_seq h' state1) (U32.v Hash.pos_whash_w) (U32.(v Hash.pos_whash_w + v Hash.size_whash_w)) in
+  (**) //reveal_h32s st_h0 == Spec_Hash.h_0);
   (**) no_upd_lemma_1 h h' state1 s5;
   (**) no_upd_lemma_1 h h' state1 s4;
   (**) no_upd_lemma_1 h h' state1 mac;
-  agile_update a state1 s5; (* s5 = opad *)
+  Hash.update a state1 s5; (* s5 = opad *)
   (**) let h'' = ST.get() in
-//  (**) assert(
-//       let st_h0 = Seq.slice (as_seq h'' state1) (U32.v Hash.pos_whash_w) (U32.(v Hash.pos_whash_w + v Hash.size_whash_w)) in
-//       reveal_h32s st_h0 == Spec_Hash.(update h_0 (reveal_sbytes (as_seq h0 s5))));
+  (**) //assert(let st_h0 = Seq.slice (as_seq h'' state1) (U32.v Hash.pos_whash_w) (U32.(v Hash.pos_whash_w + v Hash.size_whash_w)) in
+  (**) //       reveal_h32s st_h0 == Spec_Hash.(update h_0 (reveal_sbytes (as_seq h0 s5))));
   (**) no_upd_lemma_1 h' h'' state1 s4;
   (**) no_upd_lemma_1 h' h'' state1 mac;
   (**) assert(as_seq h'' s4 == as_seq hinit s4);
-  agile_update_last a state1 s4 (hash_size a);
+  Hash.update_last a state1 s4 (blockLen a +^ tagLen a);
   (**) let h''' = ST.get() in
   (**) no_upd_lemma_1 h' h'' state1 s4;
   (**) no_upd_lemma_1 h' h'' state1 mac;
   (**) assert(live h''' mac);
-  agile_finish a state1 mac; //(* s7 = hash (s5 @| s4) *)
-//  (**) let h1 = ST.get() in
-//  (**) Spec_Hash.lemma_hash_single_prepend_block (reveal_sbytes (as_seq h0 s5)) (reveal_sbytes (as_seq h0 s4));
-//  Seq.lemma_eq_intro (reveal_sbytes (as_seq h1 mac)) (Spec_Hash.hash (Seq.append (reveal_sbytes (as_seq h0 s5)) (reveal_sbytes (as_seq h0 s4))));
-//  (**) assert(reveal_sbytes (as_seq h1 mac) == Spec_Hash.hash (Seq.append (reveal_sbytes (as_seq h0 s5)) (reveal_sbytes (as_seq h0 s4))));
-  (* Pop the memory frame *)
+  Hash.extract a state1 mac; //(* s7 = hash (s5 @| s4) *)
+  (**) //let h1 = ST.get() in
+  (**) //Spec_Hash.lemma_hash_single_prepend_block (reveal_sbytes (as_seq h0 s5)) (reveal_sbytes (as_seq h0 s4));
+  (**)  //Seq.lemma_eq_intro (reveal_sbytes (as_seq h1 mac)) (Spec_Hash.hash (Seq.append (reveal_sbytes (as_seq h0 s5)) (reveal_sbytes (as_seq h0 s4))));
+  (**) //assert(reveal_sbytes (as_seq h1 mac) == Spec_Hash.hash (Seq.append (reveal_sbytes (as_seq h0 s5)) (reveal_sbytes (as_seq h0 s4))));
   (**) pop_frame ()
 
-
+(* same spec as hmac with keylen = blockLen a *)
 //#reset-options "--max_fuel 0  --z3rlimit 20"
 val hmac_core:
-  a    : alg ->
-  mac  : uint8_p  {length mac = v (hash_size a)} ->
-  key  : uint8_p  {length key = v (block_size a) /\ disjoint key mac} ->
-  data : uint8_p  {length data + v (block_size a) < pow2 32 /\ disjoint data mac /\ disjoint data key} ->
-  len  : uint32_t {length data = v len} ->
+  a: alg ->
+  tag: lbptr (tagLength a) ->
+  key: lbptr (blockLength a) {disjoint key tag} ->
+  data: bptr {length data + blockLength a < pow2 32 /\ disjoint data tag /\ disjoint data key} ->
+  datalen: UInt32.t {v datalen = length data} ->
   Stack unit
-        (requires (fun h -> live h mac /\ live h key /\ live h data))
-        (ensures  (fun h0 _ h1 -> live h1 mac /\ live h0 mac
-                             /\ live h1 key /\ live h0 key
-                             /\ live h1 data /\ live h0 data /\ modifies_1 mac h0 h1))
-//                             /\ (reveal_sbytes (as_seq h1 mac) == Spec.hmac_core (reveal_sbytes (as_seq h0 key)) (reveal_sbytes (as_seq h0 data)))))
+  (requires (fun h0 -> live h0 tag /\ live h0 key /\ live h0 data))
+  (ensures  (fun h0 _ h1 -> 
+    live h1 tag /\ live h0 tag /\
+    live h1 key /\ live h0 key /\
+    live h1 data /\ live h0 data /\ modifies_1 tag h0 h1 /\
+    as_seq h1 tag = hmac a (as_seq h0 key) (as_seq h0 data)))
+
+//#reset-options "--max_fuel 0 --z3rlimit 10"
+let xor_bytes_inplace a b len =
+  C.Loops.in_place_map2 a b len (fun x y -> UInt8.logxor x y)
+// below, we only XOR with a constant bytemask.
 
 //#reset-options "--max_fuel 0  --z3rlimit 150"
-
 let hmac_core a mac key data len =
-
-  let h00 = ST.get () in
-  (* Push a new memory frame *)
+  (**) let h00 = ST.get () in
   (**) push_frame ();
-  let h0 = ST.get () in
-
+  (**) let h0 = ST.get () in
+/// 18-03-03 avoid those and do the xor on copying?
   (* Initialize constants *)
-  let ipad = Buffer.create 0x36uy (block_size a) in
-  let opad = Buffer.create 0x5cuy (block_size a) in
-
+  let ipad = Buffer.create 0x36uy (blockLen a) in
+  let opad = Buffer.create 0x5cuy (blockLen a) in
   (**) let h1 = ST.get () in
-//  (**) assert(reveal_sbytes (as_seq h1 ipad) == Seq.create (v (block_size a)) 0x36uy);
-//  (**) assert(reveal_sbytes (as_seq h1 opad) == Seq.create (v (block_size a)) 0x5cuy);
+  (**) //assert(reveal_sbytes (as_seq h1 ipad) == Seq.create (v (blockLen a)) 0x36uy);
+  (**) //assert(reveal_sbytes (as_seq h1 opad) == Seq.create (v (blockLen a)) 0x5cuy);
 
   (* Step 2: xor "result of step 1" with ipad *)
-  xor_bytes_inplace ipad key (block_size a);
+  xor_bytes_inplace ipad key (blockLen a);
   (**) let h2 = ST.get () in
-//  (**) assert(reveal_sbytes (as_seq h2 ipad) == Spec.xor_bytes (reveal_sbytes (as_seq h1 ipad)) (reveal_sbytes (as_seq h0 key)));
+  (**) //assert(reveal_sbytes (as_seq h2 ipad) == Spec.xor_bytes (reveal_sbytes (as_seq h1 ipad)) (reveal_sbytes (as_seq h0 key)));
 
   (* Step 3: append data to "result of step 2" *)
   (* Step 4: apply Hash to "result of step 3" *)
   hmac_part1 a ipad data len; (* s2 = ipad *)
-  let s4 = Buffer.sub ipad 0ul (hash_size a) in (* Salvage memory *)
+  let s4 = Buffer.sub ipad 0ul (tagLen a) in (* Salvage memory *)
   (**) let h3 = ST.get () in
-//  (**) Seq.lemma_eq_intro (as_seq h3 (Buffer.sub ipad 0ul (hash_size a))) (Seq.slice (as_seq h3 ipad) 0 (v (hash_size a)));
-//  (**) assert(reveal_sbytes (as_seq h3 s4) == Spec_Hash.hash (Seq.append (reveal_sbytes (as_seq h2 ipad)) (reveal_sbytes (as_seq h0 data))));
-//  (**) assert(reveal_sbytes (as_seq h3 s4) == Spec_Hash.hash (Seq.append (Spec.xor_bytes (reveal_sbytes (as_seq h1 ipad)) (reveal_sbytes (as_seq h0 key))) (reveal_sbytes (as_seq h0 data))));
+  (**) //Seq.lemma_eq_intro (as_seq h3 (Buffer.sub ipad 0ul (tagLen a))) (Seq.slice (as_seq h3 ipad) 0 (tagLength a));
+  (**) //assert(reveal_sbytes (as_seq h3 s4) == Spec_Hash.hash (Seq.append (reveal_sbytes (as_seq h2 ipad)) (reveal_sbytes (as_seq h0 data))));
+  (**) //assert(reveal_sbytes (as_seq h3 s4) == Spec_Hash.hash (Seq.append (Spec.xor_bytes (reveal_sbytes (as_seq h1 ipad)) (reveal_sbytes (as_seq h0 key))) (reveal_sbytes (as_seq h0 data))));
 
   (* Step 5: xor "result of step 1" with opad *)
-  xor_bytes_inplace opad key (block_size a);
+  xor_bytes_inplace opad key (blockLen a);
   (**) let h4 = ST.get () in
-//  (**) assert(reveal_sbytes (as_seq h4 opad) == Spec.xor_bytes (reveal_sbytes (as_seq h1 opad)) (reveal_sbytes (as_seq h0 key)));
+  (**) //assert(reveal_sbytes (as_seq h4 opad) == Spec.xor_bytes (reveal_sbytes (as_seq h1 opad)) (reveal_sbytes (as_seq h0 key)));
 
   (* Step 6: append "result of step 4" to "result of step 5" *)
   (* Step 7: apply H to "result of step 6" *)
   hmac_part2 a mac opad s4; (* s5 = opad *)
   (**) let h5 = ST.get () in
-//  (**) assert(reveal_sbytes (as_seq h5 mac) == Spec.hmac_core (reveal_sbytes (as_seq h0 key)) (reveal_sbytes (as_seq h0 data)));
-
-  (* Pop the memory frame *)
+  (**) //assert(reveal_sbytes (as_seq h5 mac) == Spec.hmac_core (reveal_sbytes (as_seq h0 key)) (reveal_sbytes (as_seq h0 data)));
   (**) pop_frame ()
-
-//#reset-options "--max_fuel 0  --z3rlimit 20"
-val hmac:
-  a       : alg ->
-  mac     : uint8_p  {length mac = v (hash_size a)} ->
-  key     : uint8_p  {length key = v (block_size a) /\ disjoint key mac} ->
-  keylen  : uint32_t {v keylen = length key} ->
-  data    : uint8_p  {length data + v (block_size a) < pow2 32 /\ disjoint data mac /\ disjoint data key} ->
-  datalen : uint32_t {v datalen = length data} ->
-  Stack unit
-        (requires (fun h -> live h mac /\ live h key /\ live h data))
-        (ensures  (fun h0 _ h1 -> live h1 mac /\ live h0 mac
-                             /\ live h1 key /\ live h0 key
-                             /\ live h1 data /\ live h0 data /\ modifies_1 mac h0 h1))
-//                             /\ (reveal_sbytes (as_seq h1 mac) == Spec.hmac (reveal_sbytes (as_seq h0 key)) (reveal_sbytes (as_seq h0 data)))))
 
 //#reset-options "--max_fuel 0  --z3rlimit 25"
-let hmac a mac key keylen data datalen =
-
-  (* Push a new memory frame *)
-  (**) push_frame ();
-
-  (* Allocate memory for the wrapped key *)
-  let nkey = Buffer.create 0x00uy (block_size a) in
-
-  (* Call the key wrapping function *)
-  wrap_key a nkey key keylen;
-
-  (* Call the core HMAC function *)
-  hmac_core a mac nkey data datalen;
-
-  (* Pop the memory frame *)
-  (**) pop_frame ()
+let compute a mac key keylen data datalen =
+  push_frame (); 
+  let wrapped_key = Buffer.create 0x00uy (blockLen a) in
+  wrap_key a wrapped_key key keylen;
+  hmac_core a mac wrapped_key data datalen;
+  pop_frame ()
