secure_api/hkdf/Crypto.HKDF.fsti
@@ -1,0 +1,118 @@
+module Crypto.HKDF
+
+module ST = FStar.HyperStack.ST
+open FStar.HyperStack.All
+
+open FStar.Mul
+open FStar.Ghost
+open FStar.HyperStack
+open FStar.HyperStack.ST
+open FStar.Buffer
+open FStar.UInt32
+
+open Crypto.Hash
+open FStar.Mul
+ 
+
+/// FUNCTIONAL SPECIFICATION:
+///
+/// * extraction is just HMAC using the salt as key and the input
+///   keying materials as text.
+///
+/// * expansion does its own formatting of input key materials.
+
+open FStar.Seq 
+
+
+let rec expand0 : (
+  a: Hash.alg ->
+  prk: bseq ->
+  info: bseq ->
+  required: nat ->
+  count: nat -> 
+  last: bseq {
+    length last <= tagLength a /\
+    length info + tagLength a + 1 <= maxLength a /\
+    count < 255 /\ 
+    required <= (255 - count) * tagLength a } ->
+  lbseq required )
+= fun a prk info required count last -> 
+  let n = n + 1 in 
+  let text = last @| info @| Seq.create 1 (UInt8.uint_to_t count) in
+  let tag = Crypto.HMAC.hmac a prk text in 
+  if required <= tagLength a 
+  then fst (split tag required) 
+  else tag @| expand0 a prk info (required - tagLength a) (n+1) tag 
+
+let expand a prk info length = expand0 a prk info length 0 Seq.createEmpty
+
+
+(* 18-03-05 TBC, requires TLS libraries 
+
+/// Details specific to TLS 1.3; could move to its own module.
+/// 
+/// Since derivations depend on the concrete info,
+/// we will need to prove format injective. 
+
+let tls13_prefix: Bytes.lbytes 6 = 
+  let s = Bytes.bytes_of_string "tls_13 " in 
+  assume(Bytes.length s = 6); // a bit lame; not sure how to deal with such constants
+  s
+  
+let format: (
+  a: Hash.alg -> 
+  label: string{length (Bytes.bytes_of_string label) < 256 - 6} -> 
+  hv: bseq {length hv < 256} -> 
+  len: UInt32.t {v len <= 255 * tagLength ha} ->
+  Tot bytes )
+= 
+  fun ha label hv len ->
+  let label_bytes = tls13_prefix @| Bytes.reveal (Bytes.bytes_of_string label) in
+  // lemma_repr_bytes_values (v len);
+  // lemma_repr_bytes_values (length label_bytes);
+  // lemma_repr_bytes_values (length hv);
+  FStar.Bytes.(reveal (bytes_of_int 2 (v len) @| vlbytes 1 label_bytes @| vlbytes 1 hv)) 
+
+val expand_label: 
+  #a: Hashing.alg -> 
+  prk: hkey a -> 
+  label: string{length (bytes_of_string label) < 256 - 6} -> // -9?
+  hv: bytes{length hv < 256} -> 
+  length: nat {length <= 255 * tagLength a} -> lbseq length
+let expand_label #a prk label hv length =
+  expand prk (format a label hv length) length
+
+let expand_secret #a prk label hv = expand_label prk label hv (tagLength a)
+
+/// Details specific to QUIC; could move to its own module
+
+*)
+
+/// IMPLEMENTATION
+
+//18-03-05 TODO drop hkdf_ prefix!
+
+val hkdf_extract :
+  a       : alg13 ->
+  prk     : lbptr (tagLength a) ->
+  salt    : bptr {disjoint salt prk} -> 
+  saltlen : bptrlen salt ->
+  ikm     : bptr {disjoint ikm prk} -> 
+  ikmlen  : bptrlen ikm -> Stack unit
+  (requires (fun h0 -> 
+    live h0 prk /\ live h0 salt /\ live h0 ikm ))
+  (ensures  (fun h0 r h1 -> 
+    live h1 prk /\ modifies_1 prk h0 h1 /\
+    as_seq h1 prk = Crypto.HMAC.hmac a (as_seq h0 salt) (as_seq h0 ikm)))
+
+val hkdf_expand :
+  a       : alg13 ->
+  okm     : bptr ->
+  prk     : bptr ->
+  prklen  : bptrlen prk ->
+  info    : bptr ->
+  infolen : bptrlen info -> 
+  len     : bptrlen okm { v len <= 255 * tagLength a } ->
+  Stack unit
+  (requires (fun h0 -> live h0 okm /\ live h0 prk /\ live h0 info))
+  (ensures  (fun h0 r h1 -> live h1 okm /\ modifies_1 okm h0 h1))
