secure_api/hkdf/Crypto.HMAC.fsti
@@ -1,0 +1,42 @@
+(* Agile HMAC *)
+module Crypto.HMAC
+
+/// 18-03-03 We miss a specification, to be adapted from Hashing.HMAC
+/// 18-03-03 Do we get specialized extraction of HMAC?
+ 
+open Crypto.Hash 
+
+type bseq = Seq.seq UInt8.t 
+let lbseq (l:nat) = b:bseq {Seq.length b = l}
+
+/// Agile implementation, relying on using 3 variants of SHA2
+/// supported by HACL*.
+
+(* ghost specification *)
+val hmac: 
+  a: alg13 ->
+  key: lbseq (blockLength a) ->
+  data: bseq {Seq.length data + blockLength a <= maxLength a } ->
+  lbseq (tagLength a)
+
+open FStar.HyperStack.All
+open FStar.Buffer
+
+#reset-options "--max_fuel 0  --z3rlimit 20"
+(* implementation, relying on 3 variants of SHA2 supported by HACL*; 
+   we tolerate overlaps between tag and data.
+*)
+val compute:
+  a: alg13 ->
+  tag: lbptr (tagLength a) ->
+  key: bptr {length key + blockLength a < pow2 32 /\ disjoint key tag} -> 
+  keylen: UInt32.t {UInt32.v keylen = length key} ->
+  data: bptr {length data + blockLength a < pow2 32 /\ disjoint data key} ->
+  datalen: UInt32.t {UInt32.v datalen = length data} -> 
+  Stack unit
+  (requires (fun h0 -> live h0 tag /\ live h0 key /\ live h0 data))
+  (ensures  (fun h0 _ h1 -> 
+    live h1 tag /\ live h0 tag /\
+    live h1 key /\ live h0 key /\
+    live h1 data /\ live h0 data /\ modifies_1 tag h0 h1 /\
+    as_seq h1 tag = hmac a (as_seq h0 key) (as_seq h0 data)))
