secure_api/hkdf/Crypto.Hash.fst
@@ -1,0 +1,105 @@
+(* Selected hash functions, with an agile interface and a
+   multiplex-able implementation calling into Hacl.Hash. *)
+
+module Crypto.Hash
+
+let string_of_alg = function
+  | MD5    -> "MD5"
+  | SHA1   -> "SHA1"
+  | SHA224 -> "SHA224"
+  | SHA256 -> "SHA256"
+  | SHA384 -> "SHA384"
+  | SHA512 -> "SHA512"
+
+(*
+let acc0 = function
+  | MD5 ->  [0x67452301; 0xefcdab89; 0x98badcfe; 0x10325476] // A, B, C, D
+  | SHA1 -> [0x67452301; 0xefcdab89; 0x98badcfe; 0x10325476; 0xc3d2e1f0] // h0--h4
+  | SHA224 -> [0xc1059ed8; 0x367cd507; 0x3070dd17; 0xf70e5939; 0xffc00b31; 0x68581511; 0x64f98fa7; 0xbefa4fa4] // second 32 bits of the fractional parts of the square roots of the 9th through 16th primes 23..53
+  | SHA256 -> [0x6a09e667; 0xbb67ae85; 0x3c6ef372; 0xa54ff53a; 0x510e527f; 0x9b05688c; 0x1f83d9ab; 0x5be0cd19] // first 32 bits of the fractional parts of the square roots of the first 8 primes 2..19
+  | SHA384 -> [0xcbbb9d5dc1059ed8; 0x629a292a367cd507; 0x9159015a3070dd17; 0x152fecd8f70e5939; 0x67332667ffc00b31; 0x8eb44a8768581511; 0xdb0c2e0d64f98fa7; 0x47b5481dbefa4fa4]
+  | SHA512 -> [0x6a09e667f3bcc908; 0xbb67ae8584caa73b; 0x3c6ef372fe94f82b; 0xa54ff53a5f1d36f1; 0x510e527fade682d1; 0x9b05688c2b3e6c1f; 0x1f83d9abfb41bd6b; 0x5be0cd19137e2179]
+*)
+
+(* specification code *) 
+
+let acc a = 
+  match a with 
+  | SHA256 -> Spec.SHA2_256.block_w
+  | SHA384 -> Spec.SHA2_384.block_w
+  | SHA512 -> Spec.SHA2_512.block_w
+
+let acc0 #a = 
+  match a with 
+  | SHA256 -> Spec.SHA2_256.h_0
+  | SHA384 -> Spec.SHA2_384.h_0
+  | SHA512 -> Spec.SHA2_512.h_0
+
+let compress #a =
+  match a with 
+  | SHA256 -> Spec.SHA2_256.shuffle
+  | SHA384 -> Spec.SHA2_384.shuffle
+  | SHA512 -> Spec.SHA2_512.shuffle
+
+let finish #a  = 
+  match a with 
+  | SHA256 -> Spec.SHA2_256.finish
+  | SHA384 -> Spec.SHA2_384.finish
+  | SHA512 -> Spec.SHA2_512.finish
+
+let suffix a l = 
+  let l1 = l % blockLength a in 
+  let l0 = l - l1 in
+  match a with
+  | SHA256 -> Spec.SHA2_256.pad l0 l1
+  | SHA384 -> Spec.SHA2_384.pad l0 l1
+  | SHA512 -> Spec.SHA2_512.pad l0 l1
+
+(* implementation *) 
+
+let lemma_hash_spec a b = ()
+
+let compute a len input output = 
+  match a with
+  | SHA256 -> Hacl.Hash.SHA2_256.hash output input len
+  | SHA384 -> Hacl.Hash.SHA2_384.hash output input len
+  | SHA512 -> Hacl.Hash.SHA2_512.hash output input len
+
+let state_size a =
+  match a with 
+  | SHA256 -> Hacl.Hash.SHA2_256.size_state
+  | SHA384 -> 2ul *^ Hacl.Hash.SHA2_384.size_state
+  | SHA512 -> 2ul *^ Hacl.Hash.SHA2_512.size_state
+
+let as_acc #a h st = admit() //TODO as_seq (sub st ...)
+
+let init a = 
+ match a with
+  | SHA256 -> Hacl.Hash.SHA2_256.init 
+  | SHA384 -> Hacl.Hash.SHA2_384.init  
+  | SHA512 -> Hacl.Hash.SHA2_512.init  
+
+let update a = 
+  match a with
+  | SHA256 -> Hacl.Hash.SHA2_256.update 
+  | SHA384 -> Hacl.Hash.SHA2_384.update 
+  | SHA512 -> Hacl.Hash.SHA2_512.update 
+
+let update_multi a st blocks len = 
+  match a with
+  | SHA256 -> Hacl.Hash.SHA2_256.update_multi st blocks (len /^ blockLen SHA256)
+  | SHA384 -> Hacl.Hash.SHA2_384.update_multi st blocks (len /^ blockLen SHA384)
+  | SHA512 -> Hacl.Hash.SHA2_512.update_multi st blocks (len /^ blockLen SHA512)
+
+let update_last a st last totlen =
+  let len = totlen %^ blockLen a in 
+  match a with 
+  | SHA256 -> Hacl.Hash.SHA2_256.update_last st last len
+  | SHA384 -> Hacl.Hash.SHA2_384.update_last st last (Int.Cast.uint32_to_uint64 len)
+  | SHA512 -> Hacl.Hash.SHA2_512.update_last st last (Int.Cast.uint32_to_uint64 len)
+
+let extract a = 
+  match a with 
+  | SHA256 -> Hacl.Hash.SHA2_256.finish
+  | SHA384 -> Hacl.Hash.SHA2_384.finish 
+  | SHA512 -> Hacl.Hash.SHA2_512.finish
