secure_api/hkdf/Crypto.Hash.fsti
@@ -1,0 +1,320 @@
+(* Selected hash functions, with an agile interface and a
+   multiplex-able implementation calling into Hacl.Hash. *)
+
+module Crypto.Hash
+
+/// adapted from [tls/src/Hashing.*]
+
+open FStar.UInt32 
+open FStar.HyperStack.ST
+
+#reset-options "--initial_ifuel 2 --initial_fuel 2 --z3rlimit 50"
+
+type bseq = Seq.seq UInt8.t 
+let lbseq (l:nat) = b:bseq {Seq.length b = l}
+
+// we also have FStar's bytes and lbytes 
+
+
+(* SUPPORTED ALGORITHMS; the first 3 are still required by TLS 1.2,
+   included for legacy purpose only, and not provided by HACL*.  See
+   e.g. https://en.wikipedia.org/wiki/SHA-1 for a global comparison
+   and lengths *)
+type alg =
+  | MD5
+  | SHA1
+  | SHA224 
+  | SHA256
+  | SHA384
+  | SHA512
+//| SHAKE128 of (n:nat{n >= 8})
+//| SHAKE256 of (n:nat{n >= 16})
+
+val string_of_alg: alg -> string 
+
+(* the algorithms used in TLS 1.3; we will make security assumptions
+   only for constructions based on those. *)
+type alg13 = a:alg {a=SHA256 \/ a=SHA384 \/ a=SHA512}
+
+(* INTERNAL BLOCK SIZE, in bytes; useful to compute various lengths. *) 
+let blockLen = function
+  | MD5 | SHA1 | SHA224 | SHA256 ->  64ul
+  | SHA384 | SHA512              -> 128ul
+//| SHAKE128 _ -> 168 | SHAKE256 _ -> 136
+  
+noextract 
+let blockLength a = UInt32.v (blockLen a)
+
+let lemma_blockLengths = 
+  assert_norm(
+    blockLength SHA256 == Spec.SHA2_256.size_block /\
+    blockLength SHA384 == Spec.SHA2_384.size_block /\
+    blockLength SHA512 == Spec.SHA2_512.size_block)
+
+(* RESULT TAGS and their lengths, in bytes *)
+
+let maxTagLen = 64ul
+let tagLen (a:alg) : Tot UInt32.t =
+  match a with
+  | MD5    -> 16ul
+  | SHA1   -> 20ul
+  | SHA224 -> 28ul // truncated SHA256
+  | SHA256 -> 32ul
+  | SHA384 -> 48ul // truncated SHA512
+  | SHA512 -> 64ul
+noextract let tagLength a = v (tagLen a)
+let lemma_maxLen (a:alg) = assert_norm(tagLen a <=^ maxTagLen)
+
+// used in TLS?
+let lbytes l = b:Bytes.bytes {Bytes.length b = l}
+type tag (a:alg) = b: lbytes (tagLength a)
+type anyTag = lbytes (v maxTagLen)
+
+noextract let lemma_tagLengths = 
+  assert_norm(
+    tagLength SHA256 == Spec.SHA2_256.size_hash /\
+    // truncated SHA512; note that `size_hash` is 64, not 48
+    tagLength SHA384 == Spec.SHA2_384.(size_word `op_Multiply` size_hash_final_w) /\
+    tagLength SHA512 == Spec.SHA2_512.size_hash)
+
+//#reset-options "--initial_ifuel 2 --initial_fuel 2 --z3rlimit 30"
+(* maximal input size, in bytes *)
+noextract let maxLength: alg -> nat = function
+  // 18-03-02 hacl-star uses a strict inequality; why?
+  | SHA256 -> Spec.SHA2_256.max_input_len_8 - 1 
+  | SHA384 -> Spec.SHA2_384.max_input_len_8 - 1 
+  | SHA512 -> Spec.SHA2_512.max_input_len_8 - 1
+  | _      -> pow2 61 (* conservative *)
+noextract let lemma_maxLength (a:alg13) = assert_norm (pow2 32 <= maxLength a) 
+noextract let hashable (a:alg) = b: bseq{ Seq.length b <= maxLength a }
+
+(* MERKLE-DAMGARD algorithmic specification; not yet an incremental
+   algorithms for all byte lengths; used for aligning specs and
+   implementations but irrelevant for using hashes.  *)
+
+val acc (a:alg): Type0 (*noeq*)
+
+(* sets the initial value of the accumulator *) 
+val acc0: #a:alg -> acc a 
+
+(* hashes one block of data into the accumulator *)
+val compress: #a:alg -> acc a -> b: lbseq (blockLength a) -> acc a 
+
+(* extracts the tag from the (possibly larger) accumulator *)
+val finish: #a:alg -> acc a -> lbseq (tagLength a)
+
+// val hash2: #a:alg -> acc a -> b:bytes {length b % blockLength a = 0} -> acc a (decreases (length b))
+noextract let rec hash2 
+  (#a:alg) 
+  (v:acc a) 
+  (b:bseq {Seq.length b % blockLength a = 0}): 
+  Tot (acc a) (decreases (Seq.length b))
+=  
+  if Seq.length b = 0 then v
+  else
+    let c,b = Seq.split b (blockLength a) in
+    hash2 (compress v c) b
+
+(* PADDING AND LENGTH ENCODING *) 
+
+// for convenience, we treat inputs as sequences of bytes, not bits.
+// but note what's encoded in the suffix is the length in bits.
+private noextract
+let suffixLength (a:alg13) (length:nat {length <= maxLength a}): 
+  n:nat{ (length + n) % blockLength a = 0 /\ n <= blockLength a + 9 } 
+=
+  let blocklen = v (blockLen a) in 
+  let lenlen = match a with | SHA384 | SHA512 -> 8 | _ -> 4 in
+  let required =  length + 1 + lenlen in // minimal length after padding and encoding the length
+  let zeros = // minimal extra padding for block alignment
+    if required % blocklen = 0 
+    then 0
+    else blocklen - (required % blocklen) in
+    //was, harder to prove: required + blockLen a - ((required - 1) % blockLen a + 1) in
+  1 + zeros + lenlen
+
+val suffix: a:alg13 -> l:nat {l <= maxLength a} -> lbseq (suffixLength a l)
+
+let spec (a:alg13) (b:hashable a): lbseq (tagLength a) =
+  let blocks = Seq.append b (suffix a (Seq.length b)) in
+  let acc = hash2 acc0 blocks in
+  let tag = finish acc in
+  tag
+
+
+(* ABSTRACT, EXTERNAL SPECIFICATION *) 
+
+(*abstract*) 
+noextract 
+let hash (a:alg13) (b: hashable a): lbseq (tagLength a) = 
+  match a with 
+  | SHA256 -> Spec.SHA2_256.hash b
+  | SHA384 -> Spec.SHA2_384.hash b
+  | SHA512 -> Spec.SHA2_512.hash b
+
+// TODO? I'd rather see Spec.Hash use the simpler style above than
+// write an inductive proof.
+
+val lemma_hash_spec: a:alg13 -> b: hashable a -> Lemma (hash a b = spec a b)
+
+
+(* ONE-SHOT IMPLEMENTATION; no need for an explicit bound since len <= 2^32 *)
+
+type bptr = Buffer.buffer UInt8.t 
+let lbptr (l:nat)= b:bptr {Buffer.length b = l}
+let bptrlen (b:bptr) = len:UInt32.t {UInt32.v len = Buffer.length b}
+
+(* alternative seq, vec, ptr
+type uint8_s = Seq.seq UInt8.t
+type uint8_v = 
+type uint8_p = Buffer.buffer UInt8.t 
+*)
+
+val compute: 
+  a: alg13 -> 
+  len: UInt32.t -> 
+  input: lbptr (v len) -> 
+  output: lbptr (tagLength a){ Buffer.disjoint input output } -> Stack unit
+  (requires fun h0 -> 
+    Buffer.live h0 input /\ Buffer.live h0 output)
+  (ensures fun h0 () h1 -> 
+    Buffer.live h1 input /\ Buffer.live h1 output /\
+    Buffer.modifies_1 output h0 h1 /\
+    Buffer.as_seq h1 output = hash a (Buffer.as_seq h0 input))
+
+(* functional implementation wrapper *)
+
+// TODO missing BufferBytes here
+// val eval: a: alg13 -> b: Bytes.bytes -> Stack (Bytes.lbytes (tagLength a))
+//   (requires fun h -> True)
+//   (ensures fun h0 tag h1 -> Bytes.reveal tag = hash a (Bytes.reveal b) /\ h0 == h1)
+
+
+
+
+// TODO lowering the commented-out code in Hashing.fst 
+
+(* IMPLEMENTATION DETAILS supporting agile incremental hash, hmac, etc *)
+
+// based on Crypto.HMAC, removing the agile_ prefixes
+
+(* convenient but a bit too concrete; the caller will allocate. See also the hack in Crypto.HMAC, and the need for disjointness. *)
+
+// FIXME(adl): hash state allocation
+// The type of state a is a buffer of uint32 for SHA256
+// but a buffer of uint64 for SHA384 and SHA512
+// This is hard to do in KreMLin (see Crypto.Symmetric.PRF)
+// Instead we fake a u64[n] by allocation a u32[2*n]
+// and rely on the implicit cast in C
+val state_size: alg13 -> UInt32.t 
+
+noextract 
+let state (a:alg13) =
+  match a with
+  | SHA256 -> b:Buffer.buffer UInt32.t {Buffer.length b = v (state_size SHA256)}
+  | SHA384 -> b:Buffer.buffer UInt64.t {Buffer.length b = v ( state_size SHA384)}
+  | SHA512 -> b:Buffer.buffer UInt64.t {Buffer.length b = v (state_size SHA512)}
+val as_acc: #a:alg13 -> h:FStar.HyperStack.mem -> state a -> acc a 
+
+val init:
+  a:alg13 -> 
+  st:state a -> Stack unit 
+  (requires fun h0 -> Buffer.live #(if a = SHA256 then UInt32.t else UInt64.t) h0 st)
+  (ensures fun h0 () h1 -> 
+    Buffer.live #(if a = SHA256 then UInt32.t else UInt64.t) h1 st /\
+    Buffer.modifies_1 #(if a = SHA256 then UInt32.t else UInt64.t) st h0 h1  /\ 
+    as_acc h1 st = acc0)
+
+val update:
+  a:alg13 -> 
+  st:state a -> 
+  block: lbptr (blockLength a) {Buffer.disjoint #(if a = SHA256 then UInt32.t else UInt64.t) st block} -> 
+  Stack unit 
+  (requires fun h0 -> 
+    Buffer.live #(if a = SHA256 then UInt32.t else UInt64.t) h0 st /\ 
+    Buffer.live h0 block)
+  (ensures fun h0 () h1 -> 
+    Buffer.live #(if a = SHA256 then UInt32.t else UInt64.t) h1 st /\ 
+    Buffer.live h1 block /\
+    Buffer.modifies_1 #(if a = SHA256 then UInt32.t else UInt64.t) st h0 h1 /\ 
+    as_acc h1 st = compress (as_acc h0 st) (Buffer.as_seq h0 block))
+
+// 18-03-03 update_multi is a parametric loop best left to the
+// caller---unless we expect it to be further optimized.
+// *note change of calling convention on the length*
+val update_multi:
+  a:alg13 -> 
+  st:state a -> 
+  blocks: bptr {Buffer.length blocks % blockLength a = 0 /\ Buffer.disjoint #(if a = SHA256 then UInt32.t else UInt64.t) st blocks} -> 
+  len: UInt32.t {v len = Buffer.length blocks} -> 
+  Stack unit 
+  (requires fun h0 -> 
+    Buffer.live #(if a = SHA256 then UInt32.t else UInt64.t) h0 st /\ 
+    Buffer.live h0 blocks)
+  (ensures fun h0 () h1 -> 
+    Buffer.live #(if a = SHA256 then UInt32.t else UInt64.t) h1 st /\ 
+    Buffer.live h1 blocks /\
+    Buffer.modifies_1 #(if a = SHA256 then UInt32.t else UInt64.t) st h0 h1 /\ 
+    as_acc h1 st = hash2 (as_acc h0 st) (Buffer.as_seq h0 blocks))
+
+// 18-03-05 note the *new length-passsing convention*
+// 18-03-03 it would be simpler to let the caller keep track of lengths!
+// 18-03-03 the last block is *never* complete, so there is room for the 1st byte of padding.
+val update_last:
+  a:alg13 -> 
+  st:state a -> 
+  last: bptr {Buffer.length last <= blockLength a /\ Buffer.disjoint #(if a = SHA256 then UInt32.t else UInt64.t) st last} -> 
+  total_len: UInt32.t {Buffer.length last = v total_len % blockLength a} ->
+  Stack unit 
+  (requires fun h0 -> 
+    Buffer.live #(if a = SHA256 then UInt32.t else UInt64.t) h0 st /\ Buffer.live h0 last)
+  (ensures fun h0 () h1 -> 
+    Buffer.live #(if a = SHA256 then UInt32.t else UInt64.t) h1 st /\ Buffer.live h1 last /\
+    Buffer.modifies_1 #(if a = SHA256 then UInt32.t else UInt64.t) st h0 h1 /\ 
+    ( let l1 = v total_len % blockLength a in
+      let l0 = v total_len - l1 in 
+      forall (prior: lbseq l0). 
+      ( as_acc h0 st = hash2 acc0 prior ==>
+        finish (as_acc h1 st) = spec a (Seq.append prior (Buffer.as_seq h0 last)) )))
+
+// for HSL we'll need a variant that copies, finalizes, and extracts.
+
+// 18-03-03 can't also be named finished
+val extract: 
+  a:alg13 -> 
+  st:state a -> 
+  output: lbptr (tagLength a) {Buffer.disjoint #(if a = SHA256 then UInt32.t else UInt64.t) st output} -> 
+  Stack unit 
+  (requires fun h0 -> 
+    Buffer.live #(if a = SHA256 then UInt32.t else UInt64.t) h0 st /\ Buffer.live h0 output)
+  (ensures fun h0 () h1 -> 
+    Buffer.live #(if a = SHA256 then UInt32.t else UInt64.t) h1 st /\ Buffer.live h1 output /\
+    Buffer.modifies_1 output h0 h1 /\ 
+    Buffer.as_seq h1 output = finish (as_acc h0 st))
+
+/// INCREMENTAL HASHING (working notes)
+/// The state includes
+/// - the accumulator (one or two blocks?)
+/// - the total length of inputs (len)
+/// - a partial block containing the rest of the prior input,
+///   of length len % blockSize a.
+///
+/// To accumulate any number of bytes:
+/// - we first (conditionally) copy the start of the input to complete
+///   the partial block, and update
+/// - we loop over complete blocks from the input
+/// - we finally copy the rest to the partial block.
+///
+/// We could also use the partial block for padding and finishing
+/// (with one or two extra compressions). In this style, update_last
+/// would get a full, partially-filled block from the caller, rather
+/// than allocate its own, to be completed & compressed with 10*llll,
+/// in one or two steps.
+/// - add 1
+/// - if it won't fit, pad with 0s & compress, and reset position to 0.
+/// - pad with 0s, encode length at the end of the block & compress.
+///
+/// To fork hash chains is straightforward: just copy the state on top
+/// of the stack before finishing.
+///
+/// Can we get the compression function and the loop coded in VALE?
